\documentclass[11pt]{article}
\usepackage[margin=0.6in]{geometry}
\usepackage{amsmath}  % a standard package for math writing
\usepackage{amssymb}
\usepackage{wrapfig}
\usepackage{listings}   % include the contents of code files (avoids version issues!)
\usepackage{mathpazo} % a better font than the default, according to some
\usepackage{booktabs}  % for pretty tables
\usepackage[hidelinks]{hyperref}   % makes section links, bibliography links clickable
\usepackage{graphicx}   % include images
\usepackage{wrapfig}    % wrap text at the side of a smaller figure (don't bother doing this for your own figures)
\usepackage{bm}
\usepackage[dvipsnames]{xcolor}        % write text in pretty colors
\usepackage{multicol}
\usepackage{amsthm}

\newtheorem{theorem}{Theorem}

\date{October 21, 2021}

\renewcommand\qedsymbol{$\blacksquare$}

\title{Proof Portfolio}
\author{Anupam Bhakta}


\begin{document}
	
\maketitle

\begin{theorem}
	Let $a$ be a fixed real number. Then 
	\[\sum_{i=0}^n(a+i)=\frac{1}{2}(n+1)(2a+n)\]
	for every nonnegative integer $n$.
\end{theorem}

\begin{proof}
	We proceed by induction. \\
	Let $n = 0$ be the smallest nonnegative integer. Then,
	$$\sum_{i=0}^{0}(a+i) = a = \frac{1}{2}(0+1)(2a+0).$$
	Thus, the result holds when $n = 0$. \\
	Assume that
	$$\sum_{i=0}^k(a+i)=\frac{1}{2}(k+1)(2a+k)$$
	for a nonnegative integer $k$. We show that $\sum_{i=0}^{k+1}(a+i)=\frac{1}{2}(k+2)(2a+k+1)$. Observe that
	\begin{align}
		\sum_{i=0}^{k+1}(a+i)&= (a+k+1) + \sum_{i=0}^{k}(a+i) \\
		&=(a+k+1) + \frac{1}{2}(k+1)(2a+k) \\
		&= \frac{1}{2}(2ak + 4a + k^2 +3k +2) \\
		&=\frac{1}{2}(k+2)(2a+k+1),
	\end{align}
	where in (2), we use the Inductive Hypothesis.\\\\
	Thus, by the Principle of Mathematical Induction, we conclude that $\sum_{i=0}^n(a+i)=\frac{1}{2}(n+1)(2a+n)$ for all nonnegative integers $n$.
\end{proof}

\end{document}